@prefix : <http://www.owl-ontologies.com/ns#> .
@prefix ns: <http://www.owl-ontologies.com/ns#> .
@prefix mod: <https://w3id.org/mod#> .
@prefix owl: <http://www.w3.org/2002/07/owl#> .
@prefix rdf: <http://www.w3.org/1999/02/22-rdf-syntax-ns#> .
@prefix xml: <http://www.w3.org/XML/1998/namespace> .
@prefix xsd: <http://www.w3.org/2001/XMLSchema#> .
@prefix rdfs: <http://www.w3.org/2000/01/rdf-schema#> .
@prefix dcat: <http://www.w3.org/ns/dcat#> .
@prefix dct: <http://purl.org/dc/terms/> .
@base <http://www.owl-ontologies.com/ns#> .

<http://www.owl-ontologies.com/ns#> rdf:type owl:Ontology ;
    mod:createdWith <https://chowlk.linkeddata.es/> ;
    dct:title "Bicycle Parking Spot Ontology" ;
    dct:description "Ontology describing bicycle parking spots, integrating geospatial data such as postal code, coordinates, and administrative divisions (e.g., district, neighborhood) in line with the European Open Data Strategy." ;
    dct:creator <https://chowlk.linkeddata.es/> ;
    dct:license <https://creativecommons.org/licenses/by/4.0/> ;
    dcat:theme <http://publications.europa.eu/resource/authority/data-theme/TRAN> ;
    dct:issued "2024-05-13"^^xsd:date .

#################################################################
#    Annotation properties
#################################################################

mod:createdWith rdf:type owl:AnnotationProperty .

#################################################################
#    Object Properties
#################################################################

ns:hasEstado rdf:type owl:ObjectProperty ;
    rdfs:domain ns:BicycleParkingSpot ;
    rdfs:range ns:Estado ;
    rdfs:label "has estado" ;
    dct:description "Relates a bicycle parking spot to its current status." .

ns:hasTipoVia rdf:type owl:ObjectProperty ;
    rdfs:domain ns:BicycleParkingSpot ;
    rdfs:range ns:Via ;
    rdfs:label "has tipo via" ;
    dct:description "Indicates the type of road where the bicycle parking spot is located." .

ns:isInBarrio rdf:type owl:ObjectProperty ;
    rdfs:domain ns:BicycleParkingSpot ;
    rdfs:range ns:Barrio ;
    rdfs:label "is in barrio" ;
    dct:description "Specifies the neighborhood in which the bicycle parking spot is located." .

ns:isInDistrito rdf:type owl:ObjectProperty ;
    rdfs:domain ns:BicycleParkingSpot ;
    rdfs:range ns:Distrito ;
    rdfs:label "is in distrito" ;
    dct:description "Specifies the district where the bicycle parking spot is located." .

#################################################################
#    Data properties
#################################################################

ns:codigoPostal rdf:type owl:DatatypeProperty ;
    rdfs:label "codigo postal" ;
    dct:description "Postal code of the location where the bicycle parking spot is located." .

ns:coordenadaX rdf:type owl:DatatypeProperty ;
    rdfs:label "coordenada x" ;
    dct:description "X-coordinate for the bicycle parking spot location, based on a Cartesian coordinate system." .

ns:coordenadaY rdf:type owl:DatatypeProperty ;
    rdfs:label "coordenada y" ;
    dct:description "Y-coordinate for the bicycle parking spot location, based on a Cartesian coordinate system." .

ns:estado rdf:type owl:DatatypeProperty ;
    rdfs:label "estado" ;
    dct:description "Indicates the current operational status of the bicycle parking spot." .

ns:hasFechaInstalacion rdf:type owl:DatatypeProperty ;
    rdfs:label "has fecha instalacion" ;
    dct:description "Installation date of the bicycle parking spot." .

ns:id rdf:type owl:DatatypeProperty ;
    rdfs:label "id" ;
    dct:description "Unique identifier for the bicycle parking spot." .

ns:latitud rdf:type owl:DatatypeProperty ;
    rdfs:label "latitud" ;
    dct:description "Latitude coordinate for the bicycle parking spot location." .

ns:longitud rdf:type owl:DatatypeProperty ;
    rdfs:label "longitud" ;
    dct:description "Longitude coordinate for the bicycle parking spot location." .

ns:nombre rdf:type owl:DatatypeProperty ;
    rdfs:label "nombre" ;
    dct:description "Name of the bicycle parking spot." .

ns:poblacion rdf:type owl:DatatypeProperty ;
    rdfs:label "poblacion" ;
    dct:description "Population or locality where the bicycle parking spot is situated." .

ns:tipo rdf:type owl:DatatypeProperty ;
    rdfs:label "tipo" ;
    dct:description "Type of bicycle parking spot." .

#################################################################
#    Classes
#################################################################

ns:Barrio rdf:type owl:Class ;
    rdfs:label "Barrio" ;
    dct:description "Represents a neighborhood." .

ns:BicycleParkingSpot rdf:type owl:Class ;
    rdfs:label "Bicycle Parking Spot" ;
    dct:description "Represents a bicycle parking spot in a city." .

ns:Distrito rdf:type owl:Class ;
    rdfs:label "Distrito" ;
    dct:description "Represents a district or administrative division in a city." .

ns:Estado rdf:type owl:Class ;
    rdfs:label "Estado" ;
    dct:description "Represents the operational status of a bicycle parking spot." .

ns:Via rdf:type owl:Class ;
    rdfs:label "Via" ;
    dct:description "Represents a road or street where the bicycle parking spot is located." .