@prefix : <http://www.BiciMad.es/ontology/> .
@prefix owl: <http://www.w3.org/2002/07/owl#> .
@prefix rdf: <http://www.w3.org/1999/02/22-rdf-syntax-ns#> .
@prefix xml: <http://www.w3.org/XML/1998/namespace> .
@prefix xsd: <http://www.w3.org/2001/XMLSchema#> .
@prefix rdfs: <http://www.w3.org/2000/01/rdf-schema#> .
@prefix schema: <https://schema.org/> .
@base <http://www.BiciMad.es/ontology/> .

<http://BiciMad.es/ontology#> rdf:type owl:Ontology .

#################################################################
#    Object Properties
#################################################################


###  http://www.BiciMad.es/ontology/bikeIdentifier
:bikeIdentifier rdf:type owl:ObjectProperty ;
                rdfs:subPropertyOf owl:topObjectProperty ;
                rdfs:domain :BikeTrip ;
                rdfs:range [ rdf:type owl:Restriction ;
                             owl:onProperty owl:topDataProperty ;
                             owl:allValuesFrom xsd:integer
                           ] ;
                rdfs:comment "Identificador de la bicicleta usada en el BikeTrip. No es el identificador único del BikeTrip."@es ,
                             "Identifier of the bike used in a bike trip. It is not to be considered a unique identifier of a trip."@en ;
                rdfs:label "Bike Identifier"@en ,
                           "Identificador de la Bicicleta"@es .


###  http://www.BiciMad.es/ontology/hasLockDock
:hasLockDock rdf:type owl:ObjectProperty ;
             rdfs:subPropertyOf owl:topObjectProperty ;
             rdfs:domain :BikeTrip ;
             rdfs:range [ rdf:type owl:Restriction ;
                          owl:onProperty owl:topDataProperty ;
                          owl:allValuesFrom xsd:integer
                        ] ;
             rdfs:comment "If the bike trip ended in a Bike Station, it should have a dock associated with the locking of the bike. This value is an integer representing a the dock in the station."@en ,
                          "Si el viaje en bicicleta terminó en una Estación de Bicicletas, debe tener un puerto asociado con el bloqueo de la bicicleta. Este valor es un número entero que representa el puerto de la estación."@es ;
             rdfs:label "Has a locking dock"@en ,
                        "Tiene puerto de bloqueo"@es .


###  http://www.BiciMad.es/ontology/hasUnlockDock
:hasUnlockDock rdf:type owl:ObjectProperty ;
               rdfs:subPropertyOf owl:topObjectProperty ;
               rdfs:domain :BikeTrip ;
               rdfs:range [ rdf:type owl:Restriction ;
                            owl:onProperty owl:topDataProperty ;
                            owl:allValuesFrom xsd:integer
                          ] ;
               rdfs:comment "If the bike trip started in a Bike Station, it should have a dock associated with the unlocking of the bike. This value is an integer representing a the dock in the station."@en ,
                            "Si el viaje en bicicleta empezó en una Estación de Bicicletas, debe tener un puerto asociado con el bloqueo de la bicicleta. Este valor es un número entero que representa el puerto de la estación."@es ;
               rdfs:label "Has an unlocking dock"@en ,
                          "Tiene un puerto de desbloqueo"@es .


#################################################################
#    Classes
#################################################################

###  http://www.BiciMad.es/ontology/BikeStation
:BikeStation rdf:type owl:Class ;
             rdfs:subClassOf schema:CivicStructure ;
             rdfs:comment "A bike station."@en ,
                          "Una estación de bicicletas."@es ;
             rdfs:label "Bike Station"@en ,
                        "Estación de Bicicletas"@es .


###  http://www.BiciMad.es/ontology/BikeTrip
:BikeTrip rdf:type owl:Class ;
          rdfs:subClassOf <http://schema.org/Trip> ;
          rdfs:comment "A trip by bike between two Places."@en ,
                       "Un viaje en bicicleta."@es ;
          rdfs:label "Trip by Bike"@en ,
                     "Viaje en Bicicleta"@es .


###  Generated by the OWL API (version 4.5.29.2024-05-13T12:11:03Z) https://github.com/owlcs/owlapi
